theories/case_studies/vae/vae.v
@@ -1,0 +1,121 @@
+From iris.algebra Require Import frac.
+From iris.proofmode Require Import proofmode.
+From cap_machine Require Import rules proofmode.
+From cap_machine Require Import fetch assert.
+
+Section VAE_Main.
+  Context `{MP: MachineParameters}.
+
+
+  (*
+    PSEUDO-CODE:
+
+    init:
+      set a := 0
+      call B.adv VAE.akward
+      halt
+
+    awkward:
+      set a := 0
+      call g ()
+      set a := 1
+      call g ()
+      assert (a == 1)
+      return
+   *)
+
+  Definition VAE_main_code_init : list Word :=
+    (* set a := 0 *)
+    encodeInstrsW [Store cgp 0]
+    (* call B.adv VAE.awkward *)
+    ++ fetch_instrs 3 ca0 cs0 cs1 (* ca0 -> VAE_awkward entry point *)
+    ++ fetch_instrs 0 ct0 cs0 cs1 (* ct0 -> switcher entry point *)
+    ++ fetch_instrs 2 ct1 cs0 cs1 (* ct1 -> {B.f}_(ot_switcher)  *)
+    ++
+    encodeInstrsW [
+      Jalr cra ct0; (* jmp to entry point *)
+      Halt
+    ].
+
+  Definition VAE_main_code_f (ot_switcher : OType) : list Word :=
+    (* set a := 0 *)
+    encodeInstrsW [Store cgp 0]
+    (* call g () *)
+    ++ fetch_instrs 0 ct0 cs0 cs1 (* ct0 -> switcher entry point *)
+    ++
+    encodeInstrsW [
+      Mov cs0 cra; (* stores return-to-switcher *)
+      Mov cs1 ca0; (* stores arg_1 *)
+      Mov ct1 ca0; (* place the arg_1 in ct1 *)
+      Mov ca0 0;
+      Mov ca1 0;
+      Mov ca2 0;
+      Mov ca3 0;
+      Mov ca4 0;
+      Mov ca5 0;
+      Jalr cra ct0 (* jmp to arg_1 *)
+    ]
+    (* set a := 1 *)
+    ++ encodeInstrsW [Store cgp 1; Mov cra cs0; Mov ca0 cs1]
+    (* call g () *)
+    ++ fetch_instrs 0 ct0 cs0 cs1 (* ct0 -> switcher entry point *)
+    ++
+    encodeInstrsW [
+      Mov cs0 cra; (* stores return-to-switcher *)
+      Mov ct1 ca0; (* stores arg_1 *)
+      Mov ca0 0;
+      Mov ca1 0;
+      Jalr cra ct0; (* jmp to arg_1 *)
+
+      (* assert (a == 1) *)
+      Load ct0 cgp; (* ct0 -> a *)
+      Mov ct1 1%Z  (* ct1 -> 1 *)
+    ]
+    ++ assert_instrs 1 ct2 ct3 ct4 (* asserts that ( *ct0 = *ct1 ) *)
+    (* return cra *)
+    ++
+    encodeInstrsW [
+      Mov cra cs0; (* restores the return-to-switcher *)
+
+      (* return a *)
+      Mov ca0 0%Z;
+      Mov ca1 0%Z;
+      Mov cs0 0%Z;
+      Mov cs1 0%Z;
+      JmpCap cra
+    ].
+
+  Definition vae_main_code (ot_switcher : OType) : list Word
+    := VAE_main_code_init ++ (VAE_main_code_f ot_switcher).
+
+  Definition vae_main_data : list Word := [WInt 0].
+
+  Definition vae_main_imports
+    (b_switcher e_switcher a_cc_switcher : Addr) (ot_switcher : OType)
+    (b_assert e_assert : Addr)
+    (B_adv : Sealable)
+    (b_vae_exp_tbl e_vae_exp_tbl a_vae_exp_tbl_awkward : Addr)
+    : list Word :=
+    [
+      WSentry XSRW_ Local b_switcher e_switcher a_cc_switcher;
+      WSentry RX Global b_assert e_assert b_assert;
+      WSealed ot_switcher B_adv;
+      WSealed ot_switcher (SCap RO Global b_vae_exp_tbl e_vae_exp_tbl a_vae_exp_tbl_awkward)
+    ].
+
+  Definition vae_export_table_entries
+    (b_switcher e_switcher a_cc_switcher : Addr) (ot_switcher : OType)
+    (b_assert e_assert : Addr)
+    (B_adv : Sealable)
+    (b_vae_exp_tbl e_vae_exp_tbl a_vae_exp_tbl_awkward : Addr)
+    : list Word :=
+    [WInt (switcher.encode_entry_point 1
+             (length ((
+                    vae_main_imports
+                      b_switcher e_switcher a_cc_switcher ot_switcher
+                      b_assert e_assert B_adv
+                      b_vae_exp_tbl e_vae_exp_tbl a_vae_exp_tbl_awkward
+                  ) ++ VAE_main_code_init)))
+    ].
+
+End VAE_Main.
